theories/iris/logrel/compat_cwp/common.v
@@ -202,21 +202,21 @@ Section common.
   Lemma labels_interp_cons se inst wl F L B τs ts Φ :
     sem_env_interp F se ->
     prelude.translate_types (fc_type_vars F) τs = Some ts ->
-    (∀ fr' vs',
+    □ (∀ fr' vs',
        (frame_interp rti sr se L wl inst fr' ∗
         ∃ os' θ0, values_interp rti sr se τs os' ∗ atoms_interp os' vs' ∗ rt_token rti sr θ0) -∗
        Φ fr' vs') -∗
     labels_interp rti sr se inst wl F.(fc_labels) B -∗
     labels_interp rti sr se inst wl ((τs, L) :: F.(fc_labels)) ((length ts, Φ) :: B).
   Proof.
-    iIntros (Hse Hts) "HΦ Hlabels".
+    iIntros (Hse Hts) "#HΦ Hlabels".
     unfold labels_interp.
     unfold const.
     rewrite big_sepL2_cons.
     iSplitL "HΦ".
     - iSplitR.
       + by erewrite translate_types_comp_sem.
-      + iIntros (fr vs os θ) "Hvs Hos Hframe Hrti". iApply "HΦ". iFrame.
+      + iIntros (fr vs os θ) "!> Hvs Hos Hframe Hrti". iApply "HΦ". iFrame.
     - done.
   Qed.
 
